src/basicmodal/semantics/completeness.lean
@@ -12,80 +12,138 @@ def canonical (AX : ctx) [hax : sem_cons AX] : frame :=
   rel := λ xΓ yΔ, ∀ φ : form, □φ ∈ xΓ.val → φ ∈ yΔ.val
 }
 
-
 def val_canonical (AX : ctx) [hax : sem_cons AX] : nat → (canonical AX).states → Prop :=
   λ n, λ xΓ : (canonical AX).states, (p n) ∈ xΓ.val
-
 
 lemma existence (AX : ctx) (hax : sem_cons AX) (xΓ : (canonical AX).states) :
   ∀ φ, ◇φ ∈ xΓ.val → ∃ yΔ : (canonical AX).states, φ ∈ yΔ.val ∧ (canonical AX).rel xΓ yΔ :=
 begin
-simp, intros φ h1,
+intros φ h1,
 let Γbox : ctx := {ψ : form | □ψ ∈ xΓ.val},
-have h1 : ax_consist AX (Γbox ∪ φ), by_contradiction h2,
-have h3 : ∃ L', (∀ ψ ∈ L', ψ ∈ Γbox) ∧ prfK AX (fin_conj L' ⊃ ¬φ), 
-  from five AX Γbox φ h2,
+have h1 : ax_consist AX (Γbox ∪ {φ}), 
+{by_contradiction h2, simp at h2,
+have h3 := five AX Γbox φ h2,
 cases h3 with L h3, cases h3 with h3 h4,
-have h5 : prfK AX (□(fin_conj L ⊃ ¬φ)), from nec h4,
-have h6 : prfK AX (□(fin_conj L) ⊃ □(¬φ)), from mp kdist h5,
-simp at *, sorry, simp at *, sorry
+have h5 := cut fin_conj_boxn (mp kdist (nec h4)),
+have h6 := exercise1,
+specialize h6 xΓ.2,
+have h7 : ∀ ψ ∈ (list.map □ L), ψ ∈ xΓ.1, 
+intros ψ h8, simp at *, cases h8 with a h8,
+cases h8 with h8l h8r, specialize h3 a h8l, 
+subst h8r, exact h3,
+specialize h6 h7 h5,
+have h8 := (six AX xΓ.1 (max_imp_ax xΓ.2)).mp xΓ.2 (¬φ).box,
+cases h8 with h8l h8r, simp at *, specialize h8r h6, 
+exact absurd h1 h8r
+},
+have h2 := lindenbaum AX (Γbox ∪ {φ}) h1,
+cases h2 with Δ h2, cases h2 with h2 h3,
+let xΔ : (canonical AX).states := ⟨Δ, h2⟩,
+existsi (xΔ : (canonical AX).states),
+have h5 := set.union_subset_iff.mp h3,
+cases h5, split, simp at h5_right, exact h5_right,
+have h3 : ∀ φ : form, □φ ∈ xΓ.val → φ ∈ xΔ.val,
+intros ψ h4, apply h5_left, exact h4,
+exact h3
 end
-
 
 lemma truth (AX : ctx) (hax : sem_cons AX) (xΓ : (canonical AX).states) : 
   ∀ φ, forces (canonical AX) (val_canonical AX) xΓ φ ↔ (φ ∈ xΓ.val) :=
 begin
-intro φ, induction φ with n φ ψ ih_φ ih_ψ φ ψ ih_φ ih_ψ φ ih_φ,
+intro φ, induction φ with n φ ψ ih_φ ih_ψ 
+φ ψ ih_φ ih_ψ φ ih_φ generalizing xΓ,
 split, intro h1, exact false.elim h1,
-intro h1, 
-rw forces, 
-sorry,
-repeat {rw forces, rw val_canonical}, 
-split, intro h1, cases h1 with h1 h2, cases ih_φ,
+intro h1, rw forces, 
+have h2 := xΓ.2,
+rw max_ax_consist at h2, cases h2,
+rw ax_consist at h2_left, specialize h2_left [⊥],
+simp at *, specialize h2_left h1, 
+rw fin_ax_consist at h2_left,
+repeat {rw fin_conj at h2_left},
+exact absurd not_contra h2_left,
+repeat {rw forces, rw val_canonical},
+split, intro h1, cases h1 with h1 h2,
+specialize ih_φ xΓ, cases ih_φ,
+specialize ih_ψ xΓ,
 specialize ih_φ_mp h1, cases ih_ψ,
 specialize ih_ψ_mp h2, 
-sorry,
-intro h1, split, repeat {sorry}
+exact max_conj_1 xΓ.2 (and.intro ih_φ_mp ih_ψ_mp), 
+intro h1, split,
+specialize ih_φ xΓ, cases ih_φ, 
+apply ih_φ_mpr, exact max_conj_2 xΓ.2 h1,
+specialize ih_ψ xΓ, cases ih_ψ, 
+apply ih_ψ_mpr, exact max_conj_3 xΓ.2 h1,
+split, 
+
+intro h1, specialize ih_φ xΓ,
+specialize ih_ψ xΓ, cases ih_φ, cases ih_ψ,
+apply max_imp_1 xΓ.2,
+intro h2, specialize ih_φ_mpr h2,
+specialize h1 ih_φ_mpr, specialize ih_ψ_mp h1,
+
+exact ih_ψ_mp, 
+intros h1 h2,
+specialize ih_φ xΓ, cases ih_φ,
+specialize ih_ψ xΓ, cases ih_ψ,
+apply ih_ψ_mpr, specialize ih_φ_mp h2,
+exact max_imp_2 xΓ.2 h1 ih_φ_mp,
+split, intros h1, 
+by_contradiction h2,
+have h4 : ◇(¬φ) ∈ xΓ.val → ∃ yΔ : (canonical AX).states, 
+  (¬φ) ∈ yΔ.val ∧ (canonical AX).rel xΓ yΔ,
+from existence AX hax xΓ (¬φ),
+have h5 : (¬□(¬¬φ)) ∈ ↑xΓ, 
+{sorry},
+simp at *,
+specialize h4 h5, cases h4 with xΔ h4, cases h4 with h4 h6,
+have h7 := max_notiff AX xΔ.1 xΔ.2 φ,
+cases h7 with h7l h7r,
+specialize h7r h4, clear h7l h4 h5 h2,
+specialize ih_φ xΔ, specialize h1 xΔ h6,
+cases ih_φ, specialize ih_φ_mp h1,
+exact absurd ih_φ_mp h7r,
+intros h1 xΔ h2,
+have h3 := h2 φ h1,
+specialize ih_φ xΔ, cases ih_φ, 
+apply ih_φ_mpr, exact h3,
 end
-
-
 
 lemma comphelper (AX : ctx) (φ : form) (hax : sem_cons AX) : 
   ¬ prfK AX φ → ax_consist AX {¬φ} :=
 begin
 intro h1, rw ax_consist, intros L h2,
-rw fin_ax_consist, simp at *,
-induction L, rw fin_conj, simp, by_contradiction h3,
-have h4 : prfK AX ⊥, from mp dne h3,
-have h5 : ¬prfK AX ⊥, from nprfalse AX hax,
-exact absurd h4 h5, 
+rw fin_ax_consist, induction L, rw fin_conj, 
+by_contradiction h3,
+exact absurd (mp dne h3) (nprfalse AX hax), 
+have h4 : ∀ ψ ∈ L_hd::L_tl, ψ = ¬φ → prfK AX (¬fin_conj (L_hd::L_tl)) → prfK AX φ, 
+from fin_conj_repeat,
 simp at *, 
-cases h2 with h2 h3, subst h2,
-specialize L_ih h3, rw fin_conj,
-sorry
+cases h4 with h4 h5, cases h2 with h2 h3,
+specialize h4 h2, intro h6, apply h1, apply h4, exact h6
 end 
 
-theorem completeness (hax : sem_cons ∅) (φ : form) : 
-  global_sem_csq ∅ φ → prfK ∅ φ :=
+
+theorem completeness (AX : ctx) (hax : sem_cons AX) (φ : form) : 
+  global_sem_csq AX φ → prfK AX φ :=
 begin
 rw ←not_imp_not, intro h1,
-have h2 : ax_consist ∅ {¬φ}, from comphelper ∅ φ hax h1,
-have h3 : ∃ Γ', max_ax_consist ∅ Γ' ∧ {¬φ} ⊆ Γ', from lindenbaum ∅ {¬φ} h2,
-simp at *, cases h3 with Γ' h3, cases h3 with h3 h4, 
-rw global_sem_csq, rw not_forall, let f := canonical, use f ∅,
-rw not_forall, let v := val_canonical, use v ∅, rw not_forall,
-let xΓ' : (f ∅).states := ⟨Γ', h3⟩, use xΓ', 
-rw not_imp, split,
-intros y ψ h5, 
-have h6 : ψ ∉ ∅, {exact set.not_mem_empty ψ},
-exact absurd h5 h6,
-have h5 : forces (f ∅) (v ∅) xΓ' (¬φ) ↔ ((¬φ) ∈ xΓ'.val), 
-  from truth ∅ hax xΓ' ¬φ,
-simp at *,
+have h2 : ax_consist AX {¬φ}, from comphelper AX φ hax h1,
+have h3 : ∃ Γ', max_ax_consist AX Γ' ∧ {¬φ} ⊆ Γ', from lindenbaum AX {¬φ} h2,
+cases h3 with Γ' h3, cases h3 with h3 h4,
+rw global_sem_csq, 
+rw not_forall, let f := canonical, use f AX,
+rw not_forall, let v := val_canonical, use v AX, rw not_forall,
+let xΓ' : (f AX).states := ⟨Γ', h3⟩, use xΓ',
+rw not_imp,
+split,
+intros y ψ h5,
+sorry,
+have h5 : forces (f AX) (v AX) xΓ' (¬φ) ↔ ((¬φ) ∈ xΓ'.val), 
+  from truth AX hax xΓ' ¬φ,
 cases h5 with h5 h6,
-have h7 : ¬forces (f ∅) (v ∅) xΓ' φ ↔ forces (f ∅) (v ∅) xΓ' ¬φ, 
-  from not_forces_imp (f ∅) (v ∅) xΓ' φ,
-simp at *, cases h7 with h7 h8, apply h8, apply h6, exact h4,
+have h7 : ¬forces (f AX) (v AX) xΓ' φ ↔ forces (f AX) (v AX) xΓ' ¬φ, 
+  from not_forces_imp (f AX) (v AX) xΓ' φ,
+cases h7 with h7 h8, apply h8, apply h6, simp at *, exact h4
 end
 
 end canonical
